Making progress on the proof of Chacha20

fstar/Hacspec.Chacha20.Proof.fst
@@ -90,20 +90,190 @@ let ctr_to_seq_equiv (ctr: uint32)
   =
   assert(New.chacha20_ctr_to_seq ctr `Seq.equal #_ #1` FStar.Seq.init 1 (fun _ -> ctr))
 
-#push-options "--fuel 0 --ifuel 0 --z3rlimit 1000"
+#push-options "--z3rlimit 50"
 let chacha_block_init_equiv (key: New.key) (ctr: uint32) (iv: New.iv)
     : Lemma (New.chacha_block_init key ctr iv == Orig.chacha20_init key iv (v ctr))
   =
-  let aux (i:nat{i < 16}) : Lemma (
-    Seq.index (New.chacha_block_init key ctr iv) i ==
-    Seq.index (Orig.chacha20_init key iv (v ctr)) i
-  ) =
-    (* concat makes it hard to verify... *)
-    if i < 4 then admit()
-    else if i < 12 then admit()
-    else if i = 12 then admit()
-    else if i < 16 then admit()
-  in
-  Classical.forall_intro aux;
+  let st = Seq.create 16 (u32 0) in
+  let st = Seq.update_sub st 0 4 (Seq.map Lib.IntTypes.secret Orig.chacha20_constants) in
+  constants_equiv ();
+  assert(Seq.sub st 0 4 `Seq.equal` New.chacha20_constants_init ());
+  let st = Seq.update_sub st 4 8 (Lib.ByteSequence.uints_from_bytes_le #U32 #SEC #8 key) in
+  assert(Seq.sub st 0 4 `Seq.equal` New.chacha20_constants_init ());
+  assert(Seq.sub st 4 8 `Seq.equal` New.chacha20_key_to_u32s key);
+  let st = Seq.(st.[12] <- ctr) in
+  assert(Seq.sub st 0 4 `Seq.equal` New.chacha20_constants_init ());
+  assert(Seq.sub st 4 8 `Seq.equal` New.chacha20_key_to_u32s key);
+  assert(Seq.sub st 12 1 `Seq.equal` New.chacha20_ctr_to_seq ctr);
+  let st = Seq.update_sub st 13 3 (Lib.ByteSequence.uints_from_bytes_le #U32 #SEC #3 iv) in
+  assert(Seq.sub st 0 4 `Seq.equal` New.chacha20_constants_init ());
+  assert(Seq.sub st 4 8 `Seq.equal` New.chacha20_key_to_u32s key);
+  assert(Seq.sub st 12 1 `Seq.equal` New.chacha20_ctr_to_seq ctr);
+  assert(Seq.sub st 13 3 `Seq.equal` New.chacha20_iv_to_u32s iv);
+  assert(st `Seq.equal` Orig.chacha20_init key iv (v ctr));
   assert(New.chacha_block_init key ctr iv `Seq.equal` Orig.chacha20_init key iv (v ctr))
+#pop-options
+
+let chacha_block_inner_equiv_orig (key: New.key) (ctr: uint32) (iv: New.iv) =
+  let st0 = Orig.chacha20_init key iv (v ctr) in
+  let st = Orig.chacha20_add_counter st0 (v ctr) in
+  let st = Orig.rounds st in
+  let st = Orig.sum_state st st0 in
+  Orig.chacha20_add_counter st (v ctr)
+
+let rec repeat_left (#a: Type) (n: nat) (f: a -> a) (init: a) =
+  if n = 0 then init else repeat_left (n-1) f (f init)
+
+#push-options "--fuel 1"
+let rec repeat_left_lemma (#a: Type) (n: nat) (f: a -> a) (init: a)
+  : Lemma (f (repeat_left n f init) == repeat_left n f (f init))
+  =
+  if n = 0 then () else repeat_left_lemma (n-1) f (f init)
+#pop-options
+
+#push-options "--fuel 1"
+let rec repeat_left_equals_repeat (#a: Type) (n: nat) (f: a -> a) (init: a)
+    : Lemma (Lib.LoopCombinators.repeat n f init == repeat_left n f init)
+  =
+  if n = 0 then
+    Lib.LoopCombinators.eq_repeat0 f init
+  else begin
+    Lib.LoopCombinators.unfold_repeat n f init (n-1);
+    repeat_left_equals_repeat (n-1) f (f init);
+    repeat_left_equals_repeat (n-1) f init;
+    repeat_left_lemma (n-1) f init
+  end
+#pop-options
+
+#push-options "--fuel 1"
+let rec foldi_repeat_equiv (#a: Type) (init:a) (low: uint_size) (hi: uint_size{low <= hi})
+  (f: (i:nat{i < hi}) -> a -> a)
+  (g: a -> a)
+  (equiv: (i:nat{i < hi}) -> (x:a) -> Lemma (f i x == g x))
+    : Lemma
+      (requires (True))
+      (ensures (foldi low hi f init == Lib.LoopCombinators.repeat (hi - low) g init))
+      (decreases (hi - low))
+  =
+  if low = hi then begin
+    Lib.LoopCombinators.eq_repeat0 g init;
+    assert(foldi 0 0 f init == init)
+  end else begin
+    Lib.LoopCombinators.unfold_repeat (hi - low) g init (hi - low - 1);
+    assert(Lib.LoopCombinators.repeat (hi - low) g init ==
+      g (Lib.LoopCombinators.repeat (hi - low -1) g init));
+    (* repeat is a fold_right, whereas foldi is a fold_left. Since g and f don't depend on i
+       right or left does not matter but here we should prove that repeat is equivalent to
+       repeat_left
+    *)
+    repeat_left_equals_repeat (hi - low) g init;
+    repeat_left_equals_repeat (hi - low - 1) g (g init);
+    assert(Lib.LoopCombinators.repeat (hi - low) g init ==
+      Lib.LoopCombinators.repeat (hi - low -1) g (g init));
+    foldi_repeat_equiv (g init) (low + 1) hi f g equiv;
+    equiv low init
+  end
+#pop-options
+
+let chacha_block_inner_loop1_f = fun (i_41:uint_size{i_41 < 10})  (state_40: New.state) ->
+    let state_40 = New.chacha_double_round (state_40) in
+    (state_40)
+
+let chacha_block_inner_loop1 (state_40: New.state) =
+  foldi (usize 0) (usize 10) chacha_block_inner_loop1_f
+  (state_40)
+
+let chacha_block_inner_loop1_equiv (st: New.state)
+    : Lemma (chacha_block_inner_loop1 st == Orig.rounds st)
+  =
+  foldi_repeat_equiv st 0 10
+    chacha_block_inner_loop1_f
+    Orig.double_round (fun i x -> double_round_equiv x)
+
+let chacha_block_inner_loop2_f (st_39: New.state) =
+  fun (i_42: uint_size{i_42 < 16}) (state_40: New.state) ->
+    let state_40 =
+      array_upd #_ #16 state_40 (i_42) (
+        (array_index (state_40) (i_42)) +. (array_index (st_39) (i_42)))
+    in
+    (state_40)
+
+#push-options "--fuel 2 --z3rlimit 50"
+let rec map2_equals_foldi
+  (n: uint_size{n >= 1 /\ n <= 16})
+  (x: New.state)
+  (y: New.state)
+    : Lemma (Seq.sub (Seq.map2 (+.) x y) 0 n ==
+      Seq.sub (foldi 0 n (chacha_block_inner_loop2_f y) x) 0 n)
+  =
+  if n = 1 then begin
+    assert(Seq.sub (Seq.map2 (+.) x y) 0 n `Seq.equal`
+      Seq.sub (foldi 0 n (chacha_block_inner_loop2_f y) x) 0 n)
+  end else begin
+    map2_equals_foldi (n-1) x y;
+    assert(Seq.sub (Seq.map2 (+.) x y) 0 (n-1) `Seq.equal`
+      Seq.sub (foldi 0 (n-1) (chacha_block_inner_loop2_f y) x) 0 (n-1));
+    let aux (i: nat{i < n}) : Lemma (Seq.index (Seq.sub (Seq.map2 (+.) x y) 0 n) i ==
+      Seq.index (Seq.sub (foldi 0 n (chacha_block_inner_loop2_f y) x) 0 n) i)
+      =
+      if i < n-1 then begin
+        assert(Seq.index (Seq.sub (Seq.map2 (+.) x y) 0 n) i ==
+          Seq.index (Seq.sub (Seq.map2 (+.) x y) 0 (n-1)) i);
+        assume(Seq.index (Seq.sub (foldi 0 (n-1) (chacha_block_inner_loop2_f y) x) 0 (n-1)) i ==
+          Seq.index (Seq.sub (foldi 0 n (chacha_block_inner_loop2_f y) x) 0 n) i);
+        ()
+      end else admit()
+    in
+    Classical.forall_intro aux;
+    assert(Seq.sub (Seq.map2 (+.) x y) 0 n `Seq.equal`
+      Seq.sub (foldi 0 n (chacha_block_inner_loop2_f y) x) 0 n)
+  end
+#pop-options
+
+let chacha_block_inner_loop2 (state_40: New.state) (st_39: New.state) =
+  foldi (usize 0) (usize 16) (chacha_block_inner_loop2_f st_39) (state_40)
+
+let chacha_block_inner_loop2_equiv (st st0: New.state)
+    : Lemma (chacha_block_inner_loop2 st st0 == Orig.sum_state st st0)
+  =
+  map2_equals_foldi 16 st st0
+
+let chacha_block_inner_alt (key: New.key) (ctr: uint32) (iv: New.iv) =
+  let st = New.chacha_block_init key ctr iv in
+  let st0 = st in
+  let st = chacha_block_inner_loop1 st in
+  let st = chacha_block_inner_loop2 st st0 in
+  st
+
+let chacha_block_inner_new_comp (key: New.key) (ctr: uint32) (iv: New.iv)
+  : Lemma (New.chacha_block_inner key ctr iv == chacha_block_inner_alt key ctr iv)
+  =
+  let open FStar.Tactics in
+  assert(New.chacha_block_inner key ctr iv == chacha_block_inner_alt key ctr iv) by begin
+    norm [delta_only [
+      "Hacspec.Chacha20.chacha_block_inner";
+      "Hacspec.Chacha20.Proof.chacha_block_inner_alt";
+      "Hacspec.Chacha20.Proof.chacha_block_inner_loop1";
+      "Hacspec.Chacha20.Proof.chacha_block_inner_loop1_f";
+      "Hacspec.Chacha20.Proof.chacha_block_inner_loop2";
+      "Hacspec.Chacha20.Proof.chacha_block_inner_loop2_f"
+    ]];
+    tadmit ()
+  end
+
+#push-options "--z3rlimit 100 --fuel 0 --ifuel 0"
+let chacha_block_inner_equiv (key: New.key) (ctr: uint32) (iv: New.iv)
+    : Lemma (chacha_block_inner_alt key ctr iv == chacha_block_inner_equiv_orig key ctr iv)
+  =
+  let st = New.chacha_block_init key ctr iv in
+  let st0 = st in
+  chacha_block_init_equiv key ctr iv;
+  assert(st0 == Orig.chacha20_init key iv (v ctr));
+  let st  = chacha_block_inner_loop1 st in
+  let st = chacha_block_inner_loop2 st st0 in
+  map2_equals_foldi 16 st st0;
+  let st_orig = Orig.chacha20_add_counter st (v ctr) in
+  assume(st == chacha_block_inner_alt key ctr iv);
+  assume(st_orig == chacha_block_inner_equiv_orig key ctr iv);
+  admit()
 #pop-options
